{
 "cells": [
  {
   "cell_type": "markdown",
   "metadata": {},
   "source": [
    "# MATH50003 Numerical Analysis: Problem Sheet 9\n",
    "\n",
    "This problem sheet explores Jacobi matrices, classical orthogonal polynomials, and interpolation.\n",
    "\n",
    "Questions marked with a ‚ãÜ are meant to be completed without using a computer.\n",
    "Problems are denoted A/B/C to indicate their difficulty."
   ]
  },
  {
   "cell_type": "markdown",
   "metadata": {},
   "source": [
    "## 1. Jacobi matrices\n",
    "\n",
    "**Problem 1.1 (C)** What are the upper 3x3 sub-block of the Jacobi matrix for the \n",
    "monic and orthonormal polynomials with respect to the following weights on\n",
    "$[-1,1]$:\n",
    "$$\n",
    "1-x, \\sqrt{1-x^2}, 1-x^2\n",
    "$$"
   ]
  },
  {
   "cell_type": "markdown",
   "metadata": {},
   "source": [
    "**SOLUTION**\n",
    "\n",
    "##### Monic\n",
    "\n",
    "We know that for monic ($b_n=1$) orthogonal polynomials we can write the upper 3x3 block in the form\n",
    "\n",
    "$$X = \\begin{bmatrix} a_0 & c_0 & 0 \\\\ 1 & a_1 & c_1 \\\\ 0 & 1 & a_2 \\end{bmatrix}$$\n",
    "\n",
    "Note that for non-orthonormal polynomials the Jacobi matrix is technically the tranpose, i.e. $X^T$.\n",
    "\n",
    "1. $w(x) = 1-x$\n",
    "\n",
    "Take $p_0(x) = k_0 = 1$ (monic), then $p_1(x) = x + k_1^{(0)}$\n",
    "\n",
    "For the recurrence formula\n",
    "\n",
    "$$xp_0(x) = a_0p_0(x) + p_1(x)$$\n",
    "\n",
    "i.e. $x = a_0 + x + k_1^{(0)}$, that gives $k_1^{(0)}=-a_0$\n",
    "\n",
    "and for orthogonality, using recurrence formula and multiplying it by $p_0$ (inner product), we have\n",
    "\n",
    "$$a_0= \\frac{\\langle p_0, xp_0\\rangle}{\\|p_0\\|^2}= \\frac{\\int_{-1}^1 x(1-x) dx}{2}=-\\frac{1}{3}$$\n",
    "\n",
    "and $k_1^{(0)}=\\frac{1}{3}$\n",
    "\n",
    "For $p_2(x) = x^2 + k_2^{(1)}x+k_2^{(0)}$ we obtain\n",
    "\n",
    "$$xp_1(x)= c_0p_0(x)+a_1p_1(x)+p_2(x)$$\n",
    "\n",
    "i.e. $x^2 +\\frac{1}{3}x= c_0 + a_1x+ \\frac{1}{3}a_1 + x^2 + k_2^{(1)}x+k_2^{(0)}$, that gives $a_1+k_2^{(1)} = \\frac{1}{3}$ and $c_0+\\frac{1}{3}a_1+k_2^{(0)}=0$\n",
    "\n",
    "As before we then find\n",
    "\n",
    "$$c_0=\\frac{\\langle p_0, xp_1\\rangle}{\\|p_0\\|^2} = \\frac{\\int_{-1}^1 (x+\\frac{1}{3}) x(1-x) dx}{2}= \\frac{2}{9}$$\n",
    "\n",
    "and\n",
    "\n",
    "$$a_1 = \\frac{\\langle p_1, xp_1\\rangle}{\\|p_1\\|^2} = \\frac{\\int_{-1}^1 (x+\\frac{1}{3})^2 x(1-x) dx}{\\int_{-1}^1 (x+\\frac{1}{3})^2 (1-x) dx}= -\\frac{1}{15}$$\n",
    "\n",
    "Thus, $k_2^{(0)}= -\\frac{1}{5}$ and $k_2^{(1)}=\\frac{2}{5}$.\n",
    "\n",
    "Now\n",
    "\n",
    "$$xp_2(x)= c_1p_1(x)+a_2p_2(x)+p_3(x)$$\n",
    "\n",
    "And once again as before:\n",
    "\n",
    "$$c_1=\\frac{\\langle p_1, xp_2\\rangle}{\\|p_1\\|^2}= \\frac{\\int_{-1}^1 (x+\\frac{1}{3})(x^2+\\frac{1}{9}x- \\frac{1}{5}) x(1-x) dx}{\\int_{-1}^1 (x+\\frac{1}{3})^2 (1-x) dx}= \\frac{16}{45}$$\n",
    "\n",
    "and\n",
    "\n",
    "$$a_2 = \\frac{\\langle p_2, xp_2\\rangle}{\\|p_2\\|^2} = \\frac{\\int_{-1}^1 (x^2+\\frac{1}{9}x- \\frac{1}{5})^2 x(1-x) dx}{\\int_{-1}^1 (x^2+\\frac{1}{9}x- \\frac{1}{5})^2 (1-x) dx}= \\frac{2085}{3451}$$\n",
    "\n",
    "\n",
    "\n",
    "\n",
    "\n",
    "2. $w(x)=\\sqrt{1-x^2}$\n",
    "\n",
    "Take $p_0(x) = k_0 = 1$ (monic), then $p_1(x) = x + k_1^{(0)}$\n",
    "\n",
    "From the recurrence we have\n",
    "\n",
    "$$xp_0(x) = a_0p_0(x) + p_1(x)$$\n",
    "\n",
    "i.e. $x = a_0 + x + k_1^{(0)}$, which gives $k_1^{(0)}=-a_0$.\n",
    "\n",
    "We then proceed as before to obtain\n",
    "\n",
    "$$a_0= \\frac{\\langle p_0, xp_0\\rangle}{\\|p_0\\|^2}= \\frac{\\int_{-1}^1 x\\sqrt{1-x^2} dx}{\\pi/2}=0$$\n",
    "\n",
    "and $k_1^{(0)}=0$\n",
    "\n",
    "Likewise for $p_2(x) = x^2 + k_2^{(1)}x+k_2^{(0)}$:\n",
    "\n",
    "$$xp_1(x)= c_0p_0(x)+a_1p_1(x)+p_2(x)$$\n",
    "\n",
    "i.e. $x^2 = c_0 + a_1x + x^2 + k_2^{(1)}x+k_2^{(0)}$, which gives $a_1+k_2^{(1)} = 0$ and $c_0+k_2^{(0)}=0$\n",
    "\n",
    "Proceeding as before once again we obtain:\n",
    "\n",
    "$$c_0=\\frac{\\langle p_0, xp_1\\rangle}{\\|p_0\\|^2} \\frac{\\int_{-1}^1 x^2\\sqrt{1-x^2} dx}{\\pi/2}=\\frac{\\pi/8}{\\pi/2}= \\frac{1}{4}$$\n",
    "\n",
    "and\n",
    "\n",
    "$$a_1 = \\frac{\\langle p_1, xp_1\\rangle}{\\|p_1\\|^2} = \\frac{\\int_{-1}^1 x^3\\sqrt{1-x^2} dx}{\\int_{-1}^1 x^2 \\sqrt{1-x^2} dx}= 0$$\n",
    "\n",
    "Thus, $k_2^{(0)}= -\\frac{1}{4}$ and $k_2^{(1)}=0$.\n",
    "\n",
    "Finally:\n",
    "\n",
    "$$xp_2(x)= c_1p_1(x)+a_2p_2(x)+p_3(x)$$\n",
    "\n",
    "and thus\n",
    "\n",
    "$$c_1=\\frac{\\langle p_1, xp_2\\rangle}{\\|p_1\\|^2}= \\frac{\\int_{-1}^1 (x^2- \\frac{1}{4}) x^2\\sqrt{1-x^2} dx}{\\int_{-1}^1 x^2 \\sqrt{1-x^2} dx}= \\frac{\\pi/32}{\\pi/8}=\\frac{1}{4}$$\n",
    "\n",
    "and\n",
    "\n",
    "$$a_2 = \\frac{\\langle p_2, xp_2\\rangle}{\\|p_2\\|^2} = \\frac{\\int_{-1}^1 (x^2- \\frac{1}{4})^2 x\\sqrt{1-x^2} dx}{\\int_{-1}^1 (x^2- \\frac{1}{4})^2 \\sqrt{1-x^2} dx}= 0$$.\n",
    "\n",
    "\n",
    "\n",
    "\n",
    "3. $w(x)=1-x^2$\n",
    "\n",
    "Take $p_0(x) = k_0 = 1$ (monic), then $p_1(x) = x + k_1^{(0)}$\n",
    "\n",
    "From recurrence we have\n",
    "\n",
    "$$xp_0(x) = a_0p_0(x) + p_1(x)$$\n",
    "\n",
    "i.e. $x = a_0 + x + k_1^{(0)}$, which gives $k_1^{(0)}=-a_0$\n",
    "\n",
    "The rest works as before:\n",
    "\n",
    "$$a_0= \\frac{\\langle p_0, xp_0\\rangle}{\\|p_0\\|^2}= \\frac{\\int_{-1}^1 x(1-x^2) dx}{4/3}=0$$\n",
    "\n",
    "and $k_1^{(0)}=0$\n",
    "\n",
    "Then from\n",
    "\n",
    "$$xp_1(x)= c_0p_0(x)+a_1p_1(x)+p_2(x)$$\n",
    "\n",
    "i.e. $x^2 = c_0 + a_1x + x^2 + k_2^{(1)}x+k_2^{(0)}$, which gives $a_1+k_2^{(1)} = 0$ and $c_0+k_2^{(0)}=0$\n",
    "\n",
    "we find\n",
    "\n",
    "$$c_0=\\frac{\\langle p_0, xp_1\\rangle}{\\|p_0\\|^2} \\frac{\\int_{-1}^1 x^2(1-x^2) dx}{4/15}=\\frac{4/15}{4/3}= \\frac{1}{5}$$\n",
    "\n",
    "and\n",
    "\n",
    "$$a_1 = \\frac{\\langle p_1, xp_1\\rangle}{\\|p_1\\|^2} = \\frac{\\int_{-1}^1 x^3(1-x^2) dx}{\\int_{-1}^1 x^2 (1-x^2) dx}= 0$$\n",
    "\n",
    "i.e. $k_2^{(0)}= -\\frac{1}{5}$ and $k_2^{(1)}=0$.\n",
    "\n",
    "Finally,\n",
    "\n",
    "$$xp_2(x)= c_1p_1(x)+a_2p_2(x)+p_3(x)$$\n",
    "\n",
    "and thus\n",
    "\n",
    "$$c_1=\\frac{\\langle p_1, xp_2\\rangle}{\\|p_1\\|^2}= \\frac{\\int_{-1}^1 (x^2- \\frac{1}{5}) x^2(1-x^2) dx}{\\int_{-1}^1 x^2 (1-x^2) dx}= \\frac{32/525}{4/15}=\\frac{8}{35}$$\n",
    "\n",
    "and\n",
    "\n",
    "$$a_2 = \\frac{\\langle p_2, xp_2\\rangle}{\\|p_2\\|^2} = \\frac{\\int_{-1}^1 (x^2- \\frac{1}{4})^2 x(1-x^2) dx}{\\int_{-1}^1 (x^2- \\frac{1}{4})^2 (1-x^2) dx}= 0$$\n",
    "\n",
    "\n",
    "\n",
    "\n",
    "\n",
    "##### Orthonormal\n",
    "\n",
    "We know that for orthonormal ($b_n=c_n$) polynomials we can write the upper 3x3 block of the Jacobi matrix in the form\n",
    "\n",
    "$$X = \\begin{bmatrix} a_0 & b_0 & 0 \\\\ b_0 & a_1 & b_1 \\\\ 0 & b_1 & a_2 \\end{bmatrix}$$\n",
    "\n",
    "We could proceed step by step as above to find the entries of the recurrences but we may also take a short-cut since we already know the monic recurrence. Given any recurrence relationship coefficients $a_n, b_n, c_n$ for orthogonal polynomials for a given weight, the(symmetric) Jacobi matrix corresponding to the orthogonal polynomials for the same weight has entries $\\hat\n",
    "{b}_n = \\sqrt{c_n b_n}$ and $\\hat{a} _n = a_n$. Using this the $3 \\times 3$ blocks of the Jacobi matrices belonging to the orthonormal polynomials are straightforwardly computed from the above."
   ]
  },
  {
   "cell_type": "markdown",
   "metadata": {},
   "source": [
    "**Problem 1.2 (B)** Consider the _truncated Jacobi matrix_ associated\n",
    "with orthonormal polynomials $q_n(x)$:\n",
    "$$\n",
    "X_n := \\begin{bmatrix} a_0 & b_0 \\\\\n",
    "                         b_0 & ‚ã± & ‚ã± \\\\\n",
    "                         & ‚ã± & a_{n-2} & b_{n-2} \\\\\n",
    "                         && b_{n-2} & a_{n-1} \\end{bmatrix} ‚àà ‚Ñù^{n √ó n}\n",
    "$$\n",
    "Show that\n",
    "$$\n",
    "x [q_0(x) | ‚ãØ | q_{n-1}(x)] = [q_0(x) | ‚ãØ | q_{n-1}(x)] X_n + b_{n-1} q_n(x) ùêû_n^‚ä§.\n",
    "$$"
   ]
  },
  {
   "cell_type": "markdown",
   "metadata": {},
   "source": [
    "**SOLUTION**\n",
    "\n",
    "We have that in the infinite form of $X$:\n",
    "$$x[q_0,...,q_{n-1},...] = [q_0,...,q_{n-1},...]X$$\n",
    "\n",
    "Thus, selecting just the first $n$ terms, we have\n",
    "$$x[q_0,...,q_{n-1}] = \\left[[q_0,...,q_{n-1} ,q_n]X\\right]_{1,...,n}=\\left[[q_0,...,q_{n-1},...]X_{n+1}\\right]_{1,...,n}$$\n",
    "considering that we don't need the terms after the $n+1$ since the relevant terms in the matrix $X$ would be 0s.\n",
    "\n",
    "Writing the $n^{th}$ term explicitly we obtain\n",
    "$$xq_{n-1} = [q_{n-2},q_{n-1},q_n]\\{X_{n+1}\\}_{n,n-1:n+1}= b_{n-2}q_{n-2} + a_{n-1} q_{n-1} + b_{n-1}q_n$$\n",
    "\n",
    "While\n",
    "$$[q_{n-2},q_{n-1},q_n]\\{X_{n}\\}_{n,n-1:n+1} = b_{n-2}q_{n-2} + a_{n-1} q_{n-1}$$\n",
    "\n",
    "Thus, the only extra term that this form is missing is $b_{n-1}q_n$ in the $n^{th}$ term which can be added using the vector $e_n^T$, hence\n",
    "\n",
    "\n",
    "$$\n",
    "x [q_0(x) | ‚ãØ | q_{n-1}(x)] = [q_0(x) | ‚ãØ | q_{n-1}(x)] X_n + b_{n-1} q_n(x) ùêû_n^‚ä§\n",
    "$$"
   ]
  },
  {
   "cell_type": "markdown",
   "metadata": {},
   "source": [
    "**Problem 1.3 (A)** Prove the _Christoffel-Darboux Formula_:\n",
    "$$\n",
    "‚àë_{k = 0}^n q_k(x) q_k(y) =  b_n {q_{n+1}(x) q_n(y) - q_n(x) q_{n+1}(y) \\over x-y}\n",
    "$$\n",
    "Hint: Consider\n",
    "$$\n",
    "(x-y) [q_0(x) | ‚ãØ | q_n(x)] \\begin{bmatrix} q_0(y) \\\\ ‚ãÆ \\\\ q_n(y) \\end{bmatrix}.\n",
    "$$"
   ]
  },
  {
   "cell_type": "markdown",
   "metadata": {},
   "source": [
    "**SOLUTION**\n",
    "\n",
    "We have to prove that\n",
    "$$\n",
    "(x-y) [q_0(x) | ‚ãØ | q_n(x)] \\begin{bmatrix} q_0(y) \\\\ ‚ãÆ \\\\ q_n(y) \\end{bmatrix} = (x-y)‚àë_{k = 0}^n q_k(x) q_k(y) = b_n ({q_{n+1}(x) q_n(y) - q_n(x) q_{n+1}(y))}\n",
    "$$\n",
    "\n",
    "Using 1.2 we have\n",
    "\n",
    "$x[q_0(x) | ‚ãØ | q_n(x)] = [q_0(x) | ‚ãØ | q_n(x)] X_{n+1} + b_n q_{n+1}(x)e_{n+1}^T$\n",
    "\n",
    "$y[q_0(y) | ‚ãØ | q_n(y)] = [q_0(y) | ‚ãØ | q_n(y)] Y_{n+1} + b_n q_{n+1}(y)e_{n+1}^T$\n",
    "\n",
    "\n",
    "Right-multiplying these formulas respectively by $[q_0(y) | ‚ãØ | q_n(y)]^T$ and $[q_0(x) | ‚ãØ | q_n(x)]^T$ we obtain\n",
    "\n",
    "$x[q_0(x) | ‚ãØ | q_n(x)][q_0(y) | ‚ãØ | q_n(y)]^T = [q_0(x) | ‚ãØ | q_n(x)] X_{n+1}[q_0(y) | ‚ãØ | q_n(y)]^T + b_n q_{n+1}(x)q_n(y)$\n",
    "\n",
    "$y[q_0(y) | ‚ãØ | q_n(y)][q_0(x) | ‚ãØ | q_n(x)]^T = [q_0(y) | ‚ãØ | q_n(y)] Y_{n+1}[q_0(x) | ‚ãØ | q_n(x)]^T + b_n q_{n+1}(y)q_n(x)$\n",
    "\n",
    "which (transposed of a number) corresponds to\n",
    "\n",
    "$y[q_0(x) | ‚ãØ | q_n(x)][q_0(y) | ‚ãØ | q_n(y)]^T = [q_0(x) | ‚ãØ | q_n(x)] Y_{n+1}^T[q_0(y) | ‚ãØ | q_n(y)]^T + b_n q_n(x)q_{n+1}(y)$\n",
    "\n",
    "Subtracting from the first equation the second (transposed) we get\n",
    "\n",
    "$(x-y)[q_0(x) | ‚ãØ | q_n(x)]\\begin{bmatrix} q_0(y) \\\\ ‚ãÆ \\\\ q_n(y) \\end{bmatrix} = [q_0(x) | ‚ãØ | q_n(x)] (X_{n+1}-Y_{n+1}^T)\\begin{bmatrix} q_0(y) \\\\ ‚ãÆ \\\\ q_n(y) \\end{bmatrix} + b_n (q_{n+1}(x)q_n(y)-q_n(x)q_{n+1}(y))$\n",
    "\n",
    "But since the matrices $X_{n+1}$ and $Y_{n+1}$ do not depend on the values of $x$ and $y$, but on the polynomials, then they are the same matrix.\n",
    "\n",
    "In particular, they are symmetric matrices since the $q_k$s are orthonormal. Thus,\n",
    "$X_{n+1}-Y_{n+1}^T=0$\n",
    "\n",
    "Hence, \n",
    "$[q_0(x) | ‚ãØ | q_n(x)] (X_{n+1}-Y_{n+1}^T)\\begin{bmatrix} q_0(y) \\\\ ‚ãÆ \\\\ q_n(y) \\end{bmatrix}=0$, thus\n",
    "\n",
    "$$‚àë_{k = 0}^n q_k(x) q_k(y) = [q_0(x) | ‚ãØ | q_n(x)]\\begin{bmatrix} q_0(y) \\\\ ‚ãÆ \\\\ q_n(y) \\end{bmatrix} = { b_n (q_{n+1}(x)q_n(y)-q_n(x)q_{n+1}(y))\\over x-y}$$\n"
   ]
  },
  {
   "cell_type": "markdown",
   "metadata": {},
   "source": [
    "## 2. Chebyshev polynomials\n",
    "\n",
    "**Problem 2.1 (C)** What is the Jacobi matrix for $T_n(x)$? What scaling\n",
    "$q_n(x) = D_n T_n(x)$ gives us orthonormal polynomials?"
   ]
  },
  {
   "cell_type": "markdown",
   "metadata": {},
   "source": [
    "**SOLUTION**\n",
    "\n",
    "Let $w(x)=1/\\sqrt{1-x^2}$ on $[-1,1]$ and $q_n(x)=D_nT_n(x)$. \n",
    "\n",
    "We know $T_0(x)=1$ and we want $\\|q_0\\|=1$\n",
    "\n",
    "Thus,\n",
    "$$1=\\int_{-1}^1 D_0^2 w(x)dx = D_0^2\\pi$$\n",
    "\n",
    "Hence,\n",
    "$D_0= \\sqrt{\\frac{1}{\\pi}}$\n",
    "\n",
    "Now let $\\|q_1\\|=1$\n",
    "\n",
    "$$1=\\int_{-1}^1 D_1^2 (\\cos(acos(x)))^2 w(x)dx = D_1^2 \\int_{-1}^1 \\frac{x^2}{\\sqrt{1-x^2}}dx = D_1^2\\frac{\\pi}{2}$$\n",
    "\n",
    "Hence,\n",
    "$D_1= \\sqrt{\\frac{2}{\\pi}}$\n",
    "\n",
    "In general we want $\\|q_n\\|=1$, thus\n",
    "\n",
    "$$1=\\int_{-1}^1 D_n^2 (\\cos(n \\times acos(x)))^2 w(x)dx = D_n^2\\frac{\\pi}{2}$$\n",
    "\n",
    "Hence, $\\forall n\\ge 1$,\n",
    "$$D_n= \\sqrt{\\frac{2}{\\pi}}$$"
   ]
  },
  {
   "cell_type": "markdown",
   "metadata": {},
   "source": [
    "**Problem 2.2 (B)** Consider the function\n",
    "$$\n",
    "f(x) = \\sum_{k=0}^\\infty {T_k(x) \\over k!}\n",
    "$$\n",
    "For what coefficients $c_k$ does\n",
    "$$\n",
    "(x^2+1) f(x) = \\sum_{k=0}^\\infty c_k T_k(x)?\n",
    "$$"
   ]
  },
  {
   "cell_type": "markdown",
   "metadata": {},
   "source": [
    "**SOLUTION**\n",
    "\n",
    "We need \n",
    "\n",
    "$$(x^2+1)\\sum_{k=0}^\\infty {T_k(x) \\over k!} = \\sum_{k=0}^\\infty c_k T_k(x)$$\n",
    "\n",
    "We can use the following to rewrite the LHS\n",
    "$$xT_0(x)=T_1(x)$$\n",
    "\n",
    "$$xT_n(x)=\\frac{T_{n-1}(x)+T_{n+1}(x)}{2}$$\n",
    "\n",
    "Indeed,\n",
    "\n",
    "$$(x^2+1)\\sum_{k=0}^\\infty {T_k(x) \\over k!} = \\sum_{k=0}^\\infty {x^2T_k(x) \\over k!} + \\sum_{k=0}^\\infty {T_k(x) \\over k!} = xT_1(x)+\\sum_{k=1}^\\infty {x\\frac{T_{k-1}(x)+T_{k+1}(x)}{2 k!}} + \\sum_{k=0}^\\infty {T_k(x) \\over k!} = $$\n",
    "\n",
    "Using\n",
    "$$x\\frac{T_{0}(x)+T_{2}(x)}{2* 1!}= \\frac{T_1(x)}{2} + \\frac{T_{1}(x)+T_{3}(x)}{4}$$\n",
    "and\n",
    "$$\\sum_{k=2}^\\infty {x\\frac{T_{k-1}(x)+T_{k+1}(x)}{2 k!}}= \\sum_{k=2}^\\infty \\left(\\frac{T_{k-2}(x)+T_{k}(x)}{4k!} + \\frac{T_{k}(x)+T_{k+2}(x)}{4k!}\\right)$$\n",
    "\n",
    "\n",
    "we obtain\n",
    "\n",
    "$$= \\frac{T_{0}(x)+T_{2}(x)}{2} + \\frac{T_1(x)}{2} + \\frac{T_{1}(x)+T_{3}(x)}{4}+\\sum_{k=2}^\\infty \\left(\\frac{T_{k-2}(x)+T_{k}(x)}{4k!} + \\frac{T_{k}(x)+T_{k+2}(x)}{4k!}\\right) + \\sum_{k=0}^\\infty {T_k(x) \\over k!}$$\n",
    "\n",
    "So, we have \n",
    "\n",
    "$$c_0=\\frac{1}{2}+\\frac{1}{4*2!}+1= \\frac{13}{8}$$\n",
    "\n",
    "$$c_1=\\frac{1}{2}+\\frac{1}{4*1!}+\\frac{1}{4*3!}+1=\\frac{43}{24}$$\n",
    "\n",
    "$$c_2=\\frac{1}{2}+\\frac{2}{4*2!}+\\frac{1}{4*4!}+1$$\n",
    "\n",
    "$$c_3=\\frac{1}{4}+\\frac{2}{4*3!}+\\frac{1}{4*5!}+1$$\n",
    "\n",
    "$$c_4=\\frac{1}{4*2!}+\\frac{2}{4*4!}+\\frac{1}{4*6!}+1$$\n",
    "\n",
    "For $n\\ge3$ we have \n",
    "$$c_n=\\frac{1}{4*(n-2)!}+\\frac{1}{2*n!}+\\frac{1}{4*(n+2)!}+1$$"
   ]
  },
  {
   "cell_type": "markdown",
   "metadata": {},
   "source": [
    "\n",
    "**Problem 2.3 (B)**\n",
    "Consider orthogonal polynomials with respect to $\\sqrt{1-x^2}$ on $[0,1]$ with the\n",
    "normalisation\n",
    "$$\n",
    "U_n(x) = 2^n x^n + O(x^{n-1})\n",
    "$$\n",
    "Prove that\n",
    "$$\n",
    "U_n(\\cos Œ∏) = {\\sin(n+1) Œ∏ \\over \\sin Œ∏}\n",
    "$$\n",
    "\n",
    "**SOLUTION**\n",
    "\n",
    "We need to verify:\n",
    "1. graded polynomials\n",
    "2. orthogonal w.r.t. $\\sqrt{1-x^2}$ on $[-1,1]$, and\n",
    "3. have the leading coefficient $2^n$.\n",
    "\n",
    "(2) follows under a change of variables\n",
    "$$\\int_{-1}^1U_n(x)U_m(x)\\sqrt{1-x^2}{\\rm d}x=\\int_0^{\\pi}U_n(\\cos\\theta)U_m(\\cos\\theta)\\sin^2\\theta{\\rm d}\\theta=\\int_0^{\\pi}\\sin(n+1)\\theta\\sin(m+1)\\theta{\\rm d}\\theta=\\frac{\\pi}{2}\\delta_{mn}$$\n",
    "where the last step is a result from Fourier theories.\n",
    "\n",
    "To see that they are graded we use the fact that\n",
    "$$xU_n(x)=\\frac{\\cos\\theta\\sin(n+1)\\theta}{\\sin\\theta}=\\frac{\\sin (n+2)\\theta+\\sin n\\theta}{2\\sin\\theta}$$\n",
    "In other words $2xU_n(x)=U_{n+1}(x)+U_{n-1}(x)$. Since each time we multiply by $2x$ and $U_0(x)=1$ we have\n",
    "$$U_n(x) = 2^n x^n + O(x^{n-1})$$\n",
    "which also proves (3).\n",
    "\n",
    "\n",
    "**Problem 2.4 (B)** Show that\n",
    "$$\n",
    "\\begin{align*}\n",
    "x U_0(x) &= U_1(x)/2 \\\\\n",
    "x U_n(x) &= {U_{n-1}(x) \\over 2} + {U_{n+1}(x) \\over 2}.\n",
    "\\end{align*}\n",
    "$$\n",
    "\n",
    "**SOLUTION**\n",
    "\n",
    "The first result is trivial.\n",
    "\n",
    "To get the second result, recall that\n",
    "$$U_n(\\cos\\theta)=\\cos\\theta U_{n-1}(\\cos\\theta)+\\cos n\\theta$$\n",
    "and\n",
    "$$\\cos n\\theta=\\cos\\theta\\cos(n-1)\\theta-(1-\\cos^2\\theta)U_{n-2}(\\cos\\theta).$$\n",
    "\n",
    "The first equation gives $\\cos n\\theta$ in terms of $U_n$ and $U_{n-1}$. Substitute the result into the second equation to get\n",
    "$$U_n(x)-xU_{n-1}(x)=x(U_{n-1}(x)-xU_{n-2}(x))-(1-x^2)U_{n-2}(x)$$\n",
    "which reduces to the desired recurrence.\n",
    "\n",
    "**Problem 2.5 (C)** What is the Jacobi matrix for $U_n(x)$? What scaling\n",
    "$q_n(x) = D_n U_n(x)$ gives us orthonormal polynomials?\n",
    "\n",
    "**Solution**\n",
    "\n",
    "Problem 2.4 gives the Jacobi matrix\n",
    "$$\\begin{bmatrix}\n",
    "0 & 1/2 & \\\\\n",
    "1/2 & \\ddots & \\ddots \\\\\n",
    " & \\ddots &\n",
    "\\end{bmatrix}$$\n",
    "\n",
    "Problem 2.3 - Claim 3 gives the norms $\\|U_n\\|=\\sqrt{\\pi/2}$, so $D_n=\\sqrt{2}{\\pi}$.\n",
    "\n",
    "\n",
    "## 3. Hermite polynomials\n",
    "\n",
    "**Problem 3.1 (B)** Consider Hermite polynomials orthogonal with respect to the weight $\\exp(-x^2)$ on $‚Ñù$\n",
    "with the normalisation\n",
    "$$\n",
    "H_n(x) = 2^n x^n + O(x^{n-1}).\n",
    "$$\n",
    "Prove the Rodrigues formula\n",
    "$$\n",
    "H_n(x) = (-1)^n {{\\rm d}^n \\over {\\rm d}x^n} \\exp(-x^2)\n",
    "$$\n",
    "\n",
    "**SOLUTION**\n",
    "\n",
    "We need to verify:\n",
    "1. graded polynomials\n",
    "2. orthogonal to all lower degree polynomials on $\\mathbb{R}$, and\n",
    "3. have the right leading coefficient $2^n$.\n",
    "\n",
    "Comparing the Rodrigues formula for $n$ and $n-1$, we find that \n",
    "$$(-1)^n\\exp(-x^2)H_n(x)={{\\rm d} \\over {\\rm d}x}\\left((-1)^{n-1}\\exp(-x^2)H_{n-1}(x)\\right)$$\n",
    "which reduces to\n",
    "$$H_n(x)=2xH_{n-1}(x)-H_{n-1}'(x).$$\n",
    "\n",
    "(1) and (3) then follows from induction since $H_0(x)=1$.\n",
    "\n",
    "(2) follows by integration by parts. If $r_m$ is a degree $m<n$ polynomial we have:\n",
    "$$\\int_{-\\infty}^\\infty H_n(x)r_m(x)\\exp(-x^2){\\rm d}x=\\int_{-\\infty}^\\infty{{\\rm d}^n \\over {\\rm d}x^n} \\exp(-x^2)\\exp(-x^2){\\rm d}x=\\cdots\\text{integration by parts}\\dots=(-1)^n\\int_{-\\infty}^\\infty \\exp(-x^2)r_m^{(n)}(x)=0$$\n",
    "\n",
    "**Problem 3.2 (C)** What are $k_n^{(1)}$ and $k_n^{(2)}$ such that\n",
    "$$\n",
    "H_n(x) = 2^n x^n + k_n^{(1)} x^{n-1} + k_n^{(2)} x^{n-2} + O(x^{n-3})\n",
    "$$\n",
    "\n",
    "**SOLUTION**\n",
    "\n",
    "From Problem 3.1,\n",
    "$$H_n(x)=2xH_{n-1}(x)-H_{n-1}'(x).$$\n",
    "Thus we have\n",
    "$$k_n^{(1)}=2k_{n-1}^{(1)}$$\n",
    "$$k_n^{(2)}=2k_{n-1}^{(2)}-(n-1)2^{n-1}$$\n",
    "\n",
    "Since $k_0^{(1)}=0$, we have $k_n^{(1)}=0$. For the second recurrence, divide both sides by $2^n$:\n",
    "$$2^{-n}k_n^{(2)}=2^{-(n-1)}k_{n-1}^{(2)}-\\frac{n-1}{2}$$\n",
    "Since $k_0^{(2)}=0$, we have $2^{-n}k_n^{(2)}=-\\frac{1+\\cdots+(n-1)}{2}=-\\frac{n(n-1)}{4}$, so $k_n^{(2)}=n(n-1)2^{n-2}$.\n",
    "\n",
    "**Problem 3.3 (B)** Deduce the 3-term recurrence relationship for $H_n(x)$.\n",
    "\n",
    "**SOLUTION**\n",
    "\n",
    "Our goal is to find $a_n$, $b_n$ and $c_n$ such that\n",
    "$$xH_n(x)=c_{n-1}H_{n-1}(x)+a_nH_n(x)+b_nH_{n+1}(x).$$\n",
    "Compare the 3 leading coefficients on both sides and use the results from Problem 3.1 and Problem 3.2:\n",
    "$$2^n=0+0+b_n2^{n+1}$$\n",
    "$$0=0+a_n2^n+0$$\n",
    "$$n(n-1)2^{n-2}=c_{n-1}2^{n-1}+0+b_n(n+1)n2^{n-1}$$\n",
    "Thus we have $b_n=1/2$, $a_n=0$ and $c_{n-1}=-n$.\n",
    "\n",
    "\n",
    "\n",
    "## 4. Interpolation\n",
    "\n",
    "**Problem 4.1 (C)** Use Lagrange interpolation to\n",
    "interpolate the function $\\cos x$ by a polynomial at the points\n",
    "$[0,2,3,4]$ and evaluate at $x = 1$. \n",
    "\n",
    "**SOLUTION**\n",
    "\n",
    "- $l_0(x)=\\frac{(x-2)(x-3)(x-4)}{(0-2)(0-3)(0-4)}=-\\frac{1}{24}(x-2)(x-3)(x-4)$\n",
    "- $l_2(x)=\\frac{(x-0)(x-3)(x-4)}{(2-0)(2-3)(2-4)}=\\frac{1}{4}x(x-3)(x-4)$\n",
    "- $l_3(x)=\\frac{(x-0)(x-2)(x-4)}{(3-0)(3-2)(3-4)}=-\\frac{1}{3}x(x-2)(x-4)$\n",
    "- $l_4(x)=\\frac{(x-0)(x-2)(x-3)}{(4-0)(4-2)(4-3)}=\\frac{1}{8}x(x-2)(x-3)$\n",
    "\n",
    "$p(x)=\\cos(0)l_0(x)+\\cos(2)l_2(x)+\\cos(3)l_3(x)+\\cos(4)l_4(x)$\n",
    "\n",
    "$l_0(1)=1/4$, $l_2(1)=3/2$, $l_3(1)=-1$, $l_4(1)=1/4$, so $p(1)=1/4\\cos(0)+3/2\\cos(2)-\\cos(3)+1/4\\cos(4)$."
   ]
  },
  {
   "cell_type": "code",
   "execution_count": null,
   "metadata": {},
   "outputs": [],
   "source": [
    "using Plots\n",
    "l0(x)=-1/24*(x-2)*(x-3)*(x-4)\n",
    "l2(x)=1/4*x*(x-3)*(x-4)\n",
    "l3(x)=-1/3*x*(x-2)*(x-4)\n",
    "l4(x)=1/8*x*(x-2)*(x-3)\n",
    "p(x)=cos(0)*l0(x)+cos(2)*l2(x)+cos(3)*l3(x)+cos(4)*l4(x)\n",
    "\n",
    "plot([p cos], xlims=(-1,5))"
   ]
  },
  {
   "cell_type": "markdown",
   "metadata": {},
   "source": [
    "**Problem 4.2 (A)** Consider the re-expanding the Lagrange basis in\n",
    "monomials. Use this to construct an explicit formula for the inverse of the\n",
    "Vandermonde matrix.\n",
    "\n",
    "**SOLUTION**\n",
    "\n",
    "We use two methods to interpolate $f(x)$\n",
    "\n",
    "**Vandermonde matrix**\n",
    "\n",
    "$$p(x)=\\sum_{k=1}^nc_kx^{k-1}=\n",
    "\\underbrace{\\begin{bmatrix}\n",
    "1&x&\\cdots&x^{n-1}\n",
    "\\end{bmatrix}}_{\\mathbf{M}(x)}\n",
    "\\underbrace{\\begin{bmatrix}\n",
    "c_1\\\\\n",
    "\\vdots\\\\\n",
    "c_n\n",
    "\\end{bmatrix}}_{\\mathbf{c}}$$\n",
    "where\n",
    "$$\n",
    "V\\mathbf{c}=\n",
    "\\underbrace{\\begin{bmatrix}\n",
    "f(x_1)\\\\\n",
    "\\vdots\\\\\n",
    "f(x_n)\n",
    "\\end{bmatrix}}_{\\mathbf{f}}\n",
    "$$\n",
    "\n",
    "**Lagrange interpolation**\n",
    "\n",
    "$$p(x)=\\sum_{k=1}^nf(x_k)l_k(x)=\n",
    "\\underbrace{\\begin{bmatrix}\n",
    "l_1(x)&\\cdots&l_n(x)\n",
    "\\end{bmatrix}}_{\\mathbf{L}(x)}\\mathbf{f}$$\n",
    "\n",
    "Comparing the two results, we have\n",
    "$$\\mathbf{M}(x)V^{-1}\\mathbf{f}=\\mathbf{L}(x)\\mathbf{f},$$\n",
    "so\n",
    "$$\\mathbf{M}(x)V^{-1}=\\mathbf{L}(x)$$\n",
    "which means that the $(i,j)$-entry of $V^{-1}$ is the coefficient of $x^{i-1}$ in $l_j(x)$.\n",
    "\n",
    "See [here](https://proofwiki.org/wiki/Inverse_of_Vandermonde_Matrix#Theorem) for the complete explicit expression."
   ]
  },
  {
   "cell_type": "code",
   "execution_count": null,
   "metadata": {},
   "outputs": [],
   "source": []
  }
 ],
 "metadata": {
  "kernelspec": {
   "display_name": "Julia 1.7.1",
   "language": "julia",
   "name": "julia-1.7"
  },
  "language_info": {
   "file_extension": ".jl",
   "mimetype": "application/julia",
   "name": "julia",
   "version": "1.7.1"
  }
 },
 "nbformat": 4,
 "nbformat_minor": 2
}
